hnr_extract, hnr_frame, some steps towards hnr_RECT

HNR.thy
@@ -1,7 +1,34 @@
 theory HNR                    
-imports Sepreftime "../Imperative_HOL_Time/SepLogicTime/SepAuto"
-begin       
- 
+imports Sepreftime "../Imperative_HOL_Time/SepLogicTime/SepAuto" (* Refine_Monadic.RefineG_Recursion *)
+
+  Refine_Imperative_HOL.Structured_Apply
+begin
+
+
+lemma entailsI: 
+  assumes "\<And>h. h\<Turnstile>P \<Longrightarrow> h\<Turnstile>Q"
+  shows "P \<Longrightarrow>\<^sub>A Q" 
+  using assms unfolding entails_def by auto
+
+subsection "entailst"
+
+
+
+definition entailst :: "assn \<Rightarrow> assn \<Rightarrow> bool" (infix "\<Longrightarrow>\<^sub>t" 10)
+  where "entailst A B \<equiv> A \<Longrightarrow>\<^sub>A B * true"
+lemma enttI: "A\<Longrightarrow>\<^sub>AB*true \<Longrightarrow> A\<Longrightarrow>\<^sub>tB" unfolding entailst_def .
+lemma enttD: "A\<Longrightarrow>\<^sub>tB \<Longrightarrow> A\<Longrightarrow>\<^sub>AB*true" unfolding entailst_def .
+                                   
+lemma ent_trans[trans]: "\<lbrakk> P \<Longrightarrow>\<^sub>A Q; Q \<Longrightarrow>\<^sub>AR \<rbrakk> \<Longrightarrow> P \<Longrightarrow>\<^sub>A R"
+  by (auto intro: entailsI dest: entailsD)
+
+lemma ent_star_mono: "\<lbrakk> P \<Longrightarrow>\<^sub>A P'; Q \<Longrightarrow>\<^sub>A Q'\<rbrakk> \<Longrightarrow> P*Q \<Longrightarrow>\<^sub>A P'*Q'" 
+  using entail_trans2 entails_frame by blast
+
+lemma ent_true[simp]: "P \<Longrightarrow>\<^sub>A true" 
+  by (simp add: entails_true) 
+
+subsection "hn_refine"
 
 definition "\<And>T. hn_refine \<Gamma> c \<Gamma>' R m \<equiv> nofailT m \<longrightarrow> 
     (\<forall>h as  n   M. pHeap h as n \<Turnstile> \<Gamma>  \<longrightarrow> m = REST M \<longrightarrow>
@@ -10,17 +37,6 @@ definition "\<And>T. hn_refine \<Gamma> c \<Gamma>' R m \<equiv> nofailT m \<lon
            \<and> pHeap h' (new_addrs h as h') ((n+Ca)-t) \<Turnstile> \<Gamma>' * R ra r * true
           )
        \<and> relH {a . a < lim h \<and> a \<notin> as} h h' \<and> lim h \<le> lim h'))"    
-(*
-
-  <\<Gamma> * $T> c <\<lambda>r. \<Gamma>' * (\<exists>\<^sub>Ax. R x r * \<up>(REST [x\<mapsto>T] \<le> m)) >\<^sub>t)" 
-(* maybe T should be hidden/existentially quantified *)
-
-*)
- 
-definition hn_ctxt :: "('a\<Rightarrow>'c\<Rightarrow>assn) \<Rightarrow> 'a \<Rightarrow> 'c \<Rightarrow> assn" 
-  -- {* Tag for refinement assertion *}
-  where
-  "\<And>P. hn_ctxt P a c \<equiv> P a c"
 
 
 text "Transitivity"
@@ -40,6 +56,276 @@ lemma relH_subset:
   using assms unfolding relH_def by (auto intro: in_range_subset)
 
 
+thm entailsD
+lemma hn_refine_frame:
+  assumes "hn_refine P' c Q' R m"
+  assumes "P \<Longrightarrow>\<^sub>t F * P'"
+  shows "hn_refine P c (F * Q') R m"
+  using assms(2)
+  unfolding hn_refine_def entailst_def
+proof clarsimp
+  fix h as n M
+  assume "P \<Longrightarrow>\<^sub>A F * P' * true" "pHeap h as n \<Turnstile> P"
+  then have "pHeap h as n \<Turnstile> F * P' * true" by(rule entailsD)
+  then have H: "pHeap h as n \<Turnstile> P' * (F * true)" 
+    by (simp add: mult.assoc mult.left_commute)
+
+
+  with assms(1)[unfolded hn_refine_def] have D1: "(\<And>h as n M. pHeap h as n \<Turnstile> P' \<Longrightarrow>
+                m = SPECT M \<Longrightarrow>
+                (\<exists>h' t r. execute c h = Some (r, h', t) \<and>
+                          (\<exists>ra Ca. Some (enat Ca) \<le> M ra \<and> t \<le> n + Ca \<and> pHeap h' (new_addrs h as h') (n + Ca - t) \<Turnstile> Q' * R ra r * true) \<and>
+                          relH {a. a < heap.lim h \<and> a \<notin> as} h h' \<and> heap.lim h \<le> heap.lim h'))"
+    by auto 
+
+  from mod_star_convE[OF H]   obtain as1 as2 n1 n2 where  uni: "as = as1 \<union> as2"
+    and a: "as1 \<inter> as2 = {}" and  n: "n = n1 + n2"
+    and pH1: "pHeap h as1 n1 \<Turnstile> P'"
+    and Fr': "pHeap h as2 n2 \<Turnstile> F * true"  by blast 
+
+  assume m: "m = SPECT M"
+
+  from D1[OF pH1 m]  obtain h' t r ra Ca where
+         1: "execute c h = Some (r, h', t)" "Some (enat Ca) \<le> M ra" and 2: "t \<le> n1 + Ca"
+       and 3:                   "pHeap h' (new_addrs h as1 h') (n1 + Ca - t) \<Turnstile> Q' * R ra r * true"
+       and 4:                   "relH {a. a < heap.lim h \<and> a \<notin> as1} h h'" and 5: "heap.lim h \<le> heap.lim h'"
+    by blast
+
+  have Fr: "pHeap h' as2 n2 \<Turnstile> F * true"
+    apply(rule mod_relH[OF _ Fr'])
+    apply(rule relH_subset) apply fact  
+    using Fr' a models_in_range by fastforce 
+
+  have na: "new_addrs h as1 h' \<inter> as2 = {}" 
+    using a models_in_range[OF Fr'] 4
+    by (auto simp: new_addrs_def)
+
+  have n': "n1 + Ca - t + n2 = n + Ca - t" using n 2 by auto
+  have ne: "new_addrs h as1 h' \<union> as2 = new_addrs h as h'"
+    using uni new_addrs_def by auto 
+
+  thm mod_star_convI
+  have "pHeap h' (new_addrs h as1 h' \<union> as2) (n1 + Ca - t + n2) \<Turnstile> (Q' * R ra r * true) * (F * true)" 
+    by(rule mod_star_convI[OF na 3 Fr])  
+  then have "pHeap h' (new_addrs h as h') (n + Ca - t) \<Turnstile> (Q' * R ra r * true) * (F * true)"
+    by(simp only: n' ne)
+  then have 31: "pHeap h' (new_addrs h as h') (n + Ca - t) \<Turnstile> F * Q' * R ra r * true"
+    apply(rule entailsD[rotated]) 
+    by (simp add: assn_times_assoc entails_def mult.left_commute top_assn_reduce)   
+    
+  have 41: "relH {a. a < heap.lim h \<and> a \<notin> as} h h'"
+    apply(rule relH_subset) apply fact
+    using uni by blast
+  
+  have 21: "t \<le> n + Ca" using 2 n by auto 
+
+  from 1 21 31 41 5 show " \<exists>h' t r. execute c h = Some (r, h', t) \<and>
+                         (\<exists>ra Ca. Some (enat Ca) \<le> M ra \<and> t \<le> n + Ca \<and> pHeap h' (new_addrs h as h') (n + Ca - t) \<Turnstile> F * Q' * R ra r * true) \<and>
+                         relH {a. a < heap.lim h \<and> a \<notin> as} h h' \<and> heap.lim h \<le> heap.lim h'"
+    by auto
+qed
+ 
+lemma hnr_FAILT[simp]: "hn_refine \<Gamma> c \<Gamma>' R FAILT"
+  by(simp add: hn_refine_def)
+
+lemma pure_assn_eq_conv[simp]: "\<up>P = \<up>Q \<longleftrightarrow> P=Q" 
+  by (metis (full_types) assn_times_comm empty_iff in_range.simps mod_false' mod_pure_star_dist top_assn_rule)
+
+
+lemma hn_refine_cons_pre':
+  assumes I: "P\<Longrightarrow>\<^sub>AP' * true"
+  assumes R: "hn_refine P' c Q R m"
+  shows "hn_refine P c Q R m"
+  sorry
+
+
+
+lemma hn_refine_cons':
+  assumes I: "P\<Longrightarrow>\<^sub>AP' * true"
+  assumes R: "hn_refine P' c Q R m"
+  assumes I': "Q\<Longrightarrow>\<^sub>A Q' * true"
+  assumes R': "\<And>x y. R x y \<Longrightarrow>\<^sub>A R' x y * true"
+  shows "hn_refine P c Q' R' m"
+  using R unfolding hn_refine_def (*
+  apply clarify
+  apply (rule cons_pre_rulet[OF I])
+  apply (rule cons_post_rulet)
+  apply assumption
+  apply (sep_auto simp: entailst_def)
+  apply (rule enttD)
+  apply (intro entt_star_mono I' R')
+  done *) sorry
+
+definition hn_ctxt :: "('a\<Rightarrow>'c\<Rightarrow>assn) \<Rightarrow> 'a \<Rightarrow> 'c \<Rightarrow> assn" 
+  -- {* Tag for refinement assertion *}
+  where
+  "\<And>P. hn_ctxt P a c \<equiv> P a c"
+
+
+definition pure :: "('b \<times> 'a) set \<Rightarrow> 'a \<Rightarrow> 'b \<Rightarrow> assn"
+  -- {* Pure binding, not involving the heap *}
+  where "pure R \<equiv> (\<lambda>a c. \<up>((c,a)\<in>R))"
+
+lemma pure_app_eq: "pure R a c = \<up>((c,a)\<in>R)" by (auto simp: pure_def)
+
+lemma pure_eq_conv[simp]: "pure R = pure R' \<longleftrightarrow> R=R'"
+  unfolding pure_def 
+  apply (rule iffI)
+  apply safe
+  apply (meson pure_assn_eq_conv)
+  apply (meson pure_assn_eq_conv)
+  done
+
+lemma pure_rel_eq_false_iff: "pure R x y = false \<longleftrightarrow> (y,x)\<notin>R"
+  by (auto simp: pure_def)
+
+definition "invalid_assn R x y \<equiv> \<up>(\<exists>h. h\<Turnstile>R x y) * true"
+
+abbreviation "hn_invalid R \<equiv> hn_ctxt (invalid_assn R)"
+
+subsubsection \<open>Return\<close>
+
+
+
+lemma mod_star_trueI: "h\<Turnstile>P \<Longrightarrow> h\<Turnstile>P*true"  
+  by (metis assn_times_comm entailsD' entails_true mult.left_neutral) 
+
+
+lemma mod_false[simp]: "\<not> h\<Turnstile>false"  
+  by (simp add: pure_assn_rule)
+lemma mod_pure_star_dist[simp]: "h\<Turnstile>P*\<up>b \<longleftrightarrow> h\<Turnstile>P \<and> b"
+  by (simp add: mod_pure_star_dist)
+
+lemma f: "\<up>B * P = P * \<up>B"  
+  by (simp add: assn_times_comm)  
+lemma ff: "Q * \<up>B * P = Q * P * \<up>B"   
+  using assn_times_assoc assn_times_comm by auto  
+lemma r: "true * R   * true = R   * true"  
+  by (metis mult.assoc mult.left_commute top_assn_reduce)
+
+lemma invalidate_clone': "R x y \<Longrightarrow>\<^sub>A invalid_assn R x y * R x y * true"
+  apply (rule entailsI)
+  unfolding invalid_assn_def apply(simp add: ff f r)
+  apply (auto simp: mod_star_trueI)
+  done
+
+lemma new_addrs_id[simp]: "(new_addrs h as h) = as" unfolding new_addrs_def by auto
+  
+lemma hnr_RETURN_pass:
+  "hn_refine (hn_ctxt R x p) (return p) (hn_invalid R x p) R (REST [x\<mapsto>1])"
+  -- \<open>Pass on a value from the heap as return value\<close>
+  unfolding hn_refine_def 
+  apply (auto simp: hn_ctxt_def)
+  subgoal for h as n
+    using execute_return'[of p h] apply auto
+    subgoal  apply(rule exI[where x=1]) apply (simp add: one_enat_def) 
+      apply(rule entailsD)  by(auto  simp: invalidate_clone')   
+    subgoal by(simp add:  relH_def)  done
+  done
+
+
+lemma hnr_RETURN_pure:
+  assumes "(c,a)\<in>R"
+  shows "hn_refine emp (return c) emp (pure R) (REST [a\<mapsto>1])"
+  -- \<open>Return pure value\<close>
+  unfolding hn_refine_def 
+  apply (auto simp: hn_ctxt_def)
+  subgoal for h as n
+    using execute_return'[of c h] apply auto
+    subgoal  apply(rule exI[where x=1]) apply (simp add: one_enat_def pure_def)  
+      apply(simp add: ff f r assms)  
+      using entailsD entails_true by blast   
+    subgoal by(simp add:  relH_def)  done
+  done
+
+subsection "assert"
+
+
+definition "iASSERT ret \<Phi> \<equiv> if \<Phi> then ret () else top"
+
+definition ASSERT where "ASSERT \<equiv> iASSERT RETURNT"
+
+
+lemma bind_ASSERT_eq_if: "do { ASSERT \<Phi>; m } = (if \<Phi> then m else FAILT)"
+  unfolding ASSERT_def iASSERT_def by simp
+
+
+lemma hnr_ASSERT:
+  assumes "\<Phi> \<Longrightarrow> hn_refine \<Gamma> c \<Gamma>' R c'"
+  shows "hn_refine \<Gamma> c \<Gamma>' R (do { ASSERT \<Phi>; c'})"
+  using assms
+  apply (cases \<Phi>)
+  by(auto simp add: bind_ASSERT_eq_if) 
+
+
+subsection \<open>New command ureturn\<close>
+
+definition ureturn :: "'a \<Rightarrow> 'a Heap" where
+  [code del]: "ureturn x = Heap_Monad.heap (\<lambda>h. (x,h,0))"
+
+lemma execute_ureturn [execute_simps]:
+  "execute (ureturn x) = Some \<circ> (\<lambda>h. (x,h,0))"
+  by (simp add: ureturn_def execute_simps)
+
+lemma success_ureturnI [success_intros]:
+  "success (ureturn x) h"
+  by (rule successI) (simp add: execute_simps)
+
+lemma effect_ureturnI [effect_intros]:
+  "h = h' \<Longrightarrow> effect (ureturn x) h h' x 0"
+  by (rule effectI) (simp add: execute_simps)
+
+lemma effect_ureturnE [effect_elims]:
+  assumes "effect (ureturn x) h h' r n"
+  obtains "r = x" "h' = h" "n=0"
+  using assms by (rule effectE) (simp add: execute_simps)
+thm execute_return'
+
+lemma execute_return' [rewrite]: "execute (ureturn x) h = Some (x, h, 0)" by (metis comp_eq_dest_lhs execute_ureturn)
+
+lemma run_ureturnD: "run (ureturn x) (Some h) \<sigma> r t \<Longrightarrow> \<sigma> = Some h \<and> r = x \<and> t = 0"
+  by (auto simp add: HNR.execute_return' run.simps)
+
+lemma return_rule:
+  "<$0> ureturn x <\<lambda>r. \<up>(r = x)>" 
+  unfolding hoare_triple_def apply (auto dest!: run_ureturnD simp: timeCredit_assn_rule)
+  subgoal by (metis (mono_tags, hide_lams) pheap.sel(2) pheap.sel(3) pure_assn_rule)
+  subgoal using relH_def by fastforce 
+  done
+
+lemma hnr_uRETURN_pure:
+  assumes "(c,a)\<in>R"
+  shows "hn_refine emp (ureturn c) emp (pure R) (RETURNT a)"
+  -- \<open>Return pure value\<close>
+  unfolding hn_refine_def 
+  apply (auto simp: hn_ctxt_def)
+  subgoal for h as n
+    using execute_return'[of c h] apply auto
+    subgoal  apply(rule exI[where x=0]) apply (simp add: zero_enat_def pure_def)  
+      apply(simp add: ff f r assms)  
+      using entailsD entails_true by blast   
+    subgoal by(simp add:  relH_def)  done
+  done
+
+lemma hnr_uRETURN_pass:
+  "hn_refine (hn_ctxt R x p) (ureturn p) (hn_invalid R x p) R (RETURNT x)"
+  -- \<open>Pass on a value from the heap as return value\<close>
+  unfolding hn_refine_def 
+  apply (auto simp: hn_ctxt_def)
+  subgoal for h as n
+    using execute_return'[of p h] apply auto
+    subgoal  apply(rule exI[where x=0]) apply (simp add: zero_enat_def) 
+      apply(rule entailsD)  by(auto  simp: invalidate_clone')   
+    subgoal by(simp add:  relH_def)  done
+  done
+
+
+
+
+
+
+
+subsubsection \<open>bind\<close>
 
 
 lemma hnr_bind:
@@ -173,11 +459,263 @@ proof (goal_cases)
   qed   
 qed 
 
-lemma extract_cost_ub: "hn_refine \<Gamma> c \<Gamma>' R (REST M) \<Longrightarrow>
-      (\<And>c. c\<in>ran M \<Longrightarrow> c \<le> Cost_ub)
-      \<Longrightarrow>
-           <\<Gamma> * $Cost_ub> c <\<lambda>r. \<Gamma>' * (\<exists>\<^sub>Ara. R ra r * \<up>(ra \<in> dom M)) >\<^sub>t"
+
+
+subsubsection \<open>Recursion\<close>
+(* from Refine_Imperative_HOL.Sepref_Basic *)
+
+lemma hnr_RECT:
+  assumes S: "\<And>cf af ax px. \<lbrakk>
+    \<And>ax px. hn_refine (hn_ctxt Rx ax px * F) (cf px) (F' ax px) Ry (af ax)\<rbrakk> 
+    \<Longrightarrow> hn_refine (hn_ctxt Rx ax px * F) (cB cf px) (F' ax px) Ry (aB af ax)"
+  assumes M: "(\<And>x. mono_Heap (\<lambda>f. cB f x))"
+  shows "hn_refine 
+    (hn_ctxt Rx ax px * F) (heap.fixp_fun cB px) (F' ax px) Ry (Sepreftime.RECT aB ax)"
+  unfolding Sepreftime.RECT_def (*
+proof (simp, intro conjI impI)
+  assume "trimono aB"
+  hence "flatf_mono_ge aB" by (simp add: trimonoD)
+  have "\<forall>ax px. 
+    hn_refine (hn_ctxt Rx ax px * F) (heap.fixp_fun cB px) (F' ax px) Ry 
+      (flatf_gfp aB ax)"
+      
+    apply (rule flatf_ord.fixp_induct[OF _ \<open>flatf_mono_ge aB\<close>])  
+
+    apply (rule flatf_admissible_pointwise)
+    apply simp
+
+    apply (auto simp: hn_refine_def) [] (* have no idea what happens here ! *)
+
+    apply clarsimp
+    apply (subst heap.mono_body_fixp[of cB, OF M])
+    apply (rule S)
+    apply blast
+    done
+  thus "hn_refine (hn_ctxt Rx ax px * F)
+     (ccpo.fixp (fun_lub Heap_lub) (fun_ord Heap_ord) cB px) (F' ax px) Ry
+     (flatf_gfp aB ax)" by simp
+qed  *) sorry
+ 
+definition hor :: "assn \<Rightarrow> assn \<Rightarrow> assn" (infixr "\<or>\<^sub>A" 61)  where "hor A B = Abs_assn (Assn (
+    \<lambda>h. h\<Turnstile>A \<or> h\<Turnstile>B ) )"
+
+
+
+lemma merge_true_star[simp]: "true*true = true"
+  using top_assn_reduce by auto
+
+lemma entt_trans:
+  "entailst A B \<Longrightarrow> entailst B C \<Longrightarrow> entailst A C"
+  unfolding entailst_def
+  apply (erule ent_trans)
+  by (metis assn_times_assoc ent_star_mono ent_true merge_true_star)  
+
+lemma ent_imp_entt: "P\<Longrightarrow>\<^sub>AQ \<Longrightarrow> P\<Longrightarrow>\<^sub>tQ" 
+  apply (rule enttI)
+  apply (erule ent_trans)
+  by (simp add: entailsI mod_star_trueI)  
+
+
+lemma ent_disjI1_direct[simp]: "A \<Longrightarrow>\<^sub>A A \<or>\<^sub>A B"
   sorry
+
+lemma ent_disjI2_direct[simp]: "B \<Longrightarrow>\<^sub>A A \<or>\<^sub>A B"
+  sorry
+
+lemma entt_disjI1_direct[simp]: "A \<Longrightarrow>\<^sub>t A \<or>\<^sub>A B"
+  by (rule ent_imp_entt[OF ent_disjI1_direct])
+
+lemma entt_disjI2_direct[simp]: "B \<Longrightarrow>\<^sub>t A \<or>\<^sub>A B"
+  by (rule ent_imp_entt[OF ent_disjI2_direct])
+
+abbreviation "hn_val R \<equiv> hn_ctxt (pure R)"
+
+
+lemma hn_refine_preI: 
+  assumes "\<And>h. h\<Turnstile>\<Gamma> \<Longrightarrow> hn_refine \<Gamma> c \<Gamma>' R a"
+  shows "hn_refine \<Gamma> c \<Gamma>' R a"
+  using assms unfolding hn_refine_def (*
+  by (auto intro: hoare_triple_preI)
+   
+  *) sorry
+
+lemma entt_refl: "P\<Longrightarrow>\<^sub>t P " 
+  by (simp add: entailst_def entailsI mod_star_trueI) 
+lemma entt_refl': "P\<Longrightarrow>\<^sub>A P * true" 
+  by (simp add: entailsI mod_star_trueI) 
+
+
+lemma hn_refine_cons:
+  assumes I: "P\<Longrightarrow>\<^sub>tP'"
+  assumes R: "hn_refine P' c Q R m"
+  assumes I': "Q\<Longrightarrow>\<^sub>t Q'"
+  assumes R': "\<And>x y. R x y \<Longrightarrow>\<^sub>t R' x y"
+  shows "hn_refine P c Q' R' m" sorry
+
+lemma hn_refine_cons_post':
+  assumes R: "hn_refine P c Q R m"
+  assumes I: "Q\<Longrightarrow>\<^sub>AQ'*true"
+  shows "hn_refine P c Q' R m"
+  using assms
+  by (rule hn_refine_cons'[OF entt_refl' _ _ entt_refl'])
+
+lemma hn_refine_cons_post:
+  assumes R: "hn_refine P c Q R m"
+  assumes I: "Q\<Longrightarrow>\<^sub>tQ'"
+  shows "hn_refine P c Q' R m"
+  using assms
+  by (rule hn_refine_cons[OF entt_refl _ _ entt_refl])
+
+lemma hn_refine_split_post:
+  assumes "hn_refine \<Gamma> c \<Gamma>' R a"
+  shows "hn_refine \<Gamma> c (\<Gamma>' \<or>\<^sub>A \<Gamma>'') R a"
+  apply (rule hn_refine_cons_post[OF assms])
+  by (rule entt_disjI1_direct)
+
+
+lemma hn_refine_post_other: 
+  assumes "hn_refine \<Gamma> c \<Gamma>'' R a"
+  shows "hn_refine \<Gamma> c (\<Gamma>' \<or>\<^sub>A \<Gamma>'') R a"
+  apply (rule hn_refine_cons_post[OF assms])
+  by (rule entt_disjI2_direct)
+
+
+lemma hn_refine_cons_pre:
+  assumes I: "P\<Longrightarrow>\<^sub>tP'"
+  assumes R: "hn_refine P' c Q R m"
+  shows "hn_refine P c Q R m"
+  sorry
+
+
+lemma hnr_If':
+  assumes P: "\<Gamma> \<Longrightarrow>\<^sub>A \<Gamma>1 * hn_val bool_rel a a' * true"
+  assumes RT: "a \<Longrightarrow> hn_refine (\<Gamma>1 * hn_val bool_rel a a') b' \<Gamma>2b R b"
+  assumes RE: "\<not>a \<Longrightarrow> hn_refine (\<Gamma>1 * hn_val bool_rel a a') c' \<Gamma>2c R c"
+  assumes IMP: "\<Gamma>2b \<or>\<^sub>A \<Gamma>2c \<Longrightarrow>\<^sub>A \<Gamma>' * true"
+  shows "hn_refine \<Gamma> (if a' then b' else c') \<Gamma>' R (if a then b else c)"
+  apply (rule hn_refine_cons'[OF P])
+  apply (rule hn_refine_preI)
+  apply (cases a; simp add: hn_ctxt_def pure_def)
+     
+      apply  (rule hn_refine_split_post)
+      apply  (rule hn_refine_cons_pre'[OF _ RT])
+        apply  (simp add: hn_ctxt_def pure_def entt_refl')
+      apply  simp 
+
+    apply (rule hn_refine_post_other)
+    apply (rule hn_refine_cons_pre'[OF _ RE])
+        apply (simp add: hn_ctxt_def pure_def entt_refl')
+      apply  simp  
+  apply  (rule IMP)
+  apply  (rule entt_refl')
+  done 
+
+
+lemma hnr_If:
+  assumes P: "\<Gamma> \<Longrightarrow>\<^sub>t \<Gamma>1 * hn_val bool_rel a a'"
+  assumes RT: "a \<Longrightarrow> hn_refine (\<Gamma>1 * hn_val bool_rel a a') b' \<Gamma>2b R b"
+  assumes RE: "\<not>a \<Longrightarrow> hn_refine (\<Gamma>1 * hn_val bool_rel a a') c' \<Gamma>2c R c"
+  assumes IMP: "\<Gamma>2b \<or>\<^sub>A \<Gamma>2c \<Longrightarrow>\<^sub>t \<Gamma>'"
+  shows "hn_refine \<Gamma> (if a' then b' else c') \<Gamma>' R (if a then b else c)"
+  apply (rule hn_refine_cons[OF P])
+  apply1 (rule hn_refine_preI)
+  applyF (cases a; simp add: hn_ctxt_def pure_def)
+    focus
+      apply1 (rule hn_refine_split_post)
+        applyF (rule hn_refine_cons_pre[OF _ RT])
+        applyS (simp add: hn_ctxt_def pure_def entt_refl)
+        applyS simp
+      solved
+    solved
+    apply1 (rule hn_refine_post_other)
+    applyF (rule hn_refine_cons_pre[OF _ RE])
+      applyS (simp add: hn_ctxt_def pure_def entt_refl)
+      applyS simp
+    solved
+  solved
+  applyS (rule IMP)
+  applyS (rule entt_refl)
+  done
+
+
+lemma extract_cost_ub:
+  assumes "hn_refine \<Gamma> c \<Gamma>' R (REST M)" "(\<And>c. c\<in>ran M \<Longrightarrow> c \<le> Cost_ub)"
+  shows "<\<Gamma> * $Cost_ub> c <\<lambda>r. \<Gamma>' * (\<exists>\<^sub>Ara. R ra r * \<up>(ra \<in> dom M)) >\<^sub>t"
+  using assms(1)  unfolding hn_refine_def
+  unfolding hoare_triple_def 
+  apply clarify
+proof (goal_cases)
+  case (1 h as \<sigma> r n t)
+  from 1(2) have 2: "pHeap h as (n-Cost_ub) \<Turnstile> \<Gamma>" and  nf: "n\<ge>Cost_ub"
+    using mod_timeCredit_dest by auto
+
+  from 1(1) have 3: "\<And>h as n Ma.
+       pHeap h as n \<Turnstile> \<Gamma> \<Longrightarrow> 
+      SPECT M = SPECT Ma \<Longrightarrow> (\<exists>h' t r. execute c h = Some (r, h', t) \<and>      
+       (\<exists>ra Ca. Ma ra \<ge> Some (enat Ca) \<and> t \<le> n + Ca \<and> pHeap h' (new_addrs h as h') ((n + Ca) - t) \<Turnstile> \<Gamma>' * R ra r * true) \<and>
+      relH {a. a < heap.lim h \<and> a \<notin> as} h h' \<and> heap.lim h \<le> heap.lim h')" 
+    by auto
+
+  thm effect_deterministic
+
+  from 3[OF 2 ] obtain h' t' r' where E: "execute c h = Some (r', h', t') " and
+    R:  "(\<exists>ra Ca. M ra \<ge> Some (enat Ca) \<and>
+                    pHeap h' (new_addrs h as h') (n - Cost_ub + Ca - t') \<Turnstile> \<Gamma>' * R ra r' * true \<and> t' \<le> n - Cost_ub + Ca) \<and>
+           relH {a. a < heap.lim h \<and> a \<notin> as} h h' \<and> heap.lim h \<le> heap.lim h'" by blast
+
+  have F: "\<sigma> = Some h'" and prime: "r' = r" "t' = t"  
+    using E 1(3) run.cases apply force
+    using E 1(3) run.cases apply force
+    using E 1(3) run.cases by force 
+  then have sig: "the \<sigma> = h'" by auto
+  from R  have
+    B: "(\<exists>ra Ca. M ra \<ge> Some (enat Ca) \<and>
+     pHeap (the \<sigma>) (new_addrs h as (the \<sigma>)) (n - Cost_ub + Ca - t) \<Turnstile> \<Gamma>' * R ra r * true \<and>
+        t \<le> n - Cost_ub + Ca )" and C:
+    "relH {a. a < heap.lim h \<and> a \<notin> as} h (the \<sigma>)" "heap.lim h \<le> heap.lim (the \<sigma>) " 
+    unfolding prime sig by auto
+
+
+
+  from B obtain ra Ca where i: "pHeap (the \<sigma>) (new_addrs h as (the \<sigma>)) (n - Cost_ub + Ca - t) \<Turnstile> \<Gamma>' * R ra r * true"
+    and ii:  "t \<le> n - Cost_ub + Ca"  and ineq: "M ra \<ge> Some (enat Ca)"
+    using B by auto
+
+  from ineq have radom: "ra \<in> dom M" using domIff by fastforce  
+  then obtain Mra where Mra: "M ra = Some Mra" by blast
+  with assms(2) have "Mra \<le> enat Cost_ub" by (meson ranI)
+  with Mra ineq have "Some (enat Ca) \<le> Some (enat Cost_ub)" 
+    using dual_order.trans by fastforce 
+  then have ie: "Ca \<le> Cost_ub" by auto
+
+  have pr: "(n - Cost_ub + Ca - t) = (n - t) - (Cost_ub - Ca)" using ie ii nf by auto
+  have pl: "(n - (t + (Cost_ub - Ca)) + (Cost_ub - Ca)) = n-t" using ii nf by auto
+
+  have "pHeap (the \<sigma>) (new_addrs h as (the \<sigma>) \<union> {}) ((n - t) - (Cost_ub - Ca) + (Cost_ub - Ca)) \<Turnstile> \<Gamma>' * R ra r * true * true"
+    apply(rule mod_star_convI)  apply simp
+     apply(rule i[unfolded pr])  by (simp add: top_assn_rule)
+
+  then have H: "pHeap (the \<sigma>) (new_addrs h as (the \<sigma>)) (n - t) \<Turnstile> \<Gamma>' * R ra r * true * true"
+    by (simp add: pl)   
+
+  have "pHeap (the \<sigma>) (new_addrs h as (the \<sigma>)) (n - t) \<Turnstile> \<Gamma>' * R ra r * \<up> (ra \<in> dom M) * true"
+    apply(rule entailsD[OF _ H]) using radom by auto2  
+  then have "\<exists>ra. pHeap (the \<sigma>) (new_addrs h as (the \<sigma>)) (n - t) \<Turnstile> \<Gamma>' * R ra r * \<up> (ra \<in> dom M) * true"
+    by blast
+  then have H': "pHeap (the \<sigma>) (new_addrs h as (the \<sigma>)) (n - t) \<Turnstile> (\<exists>\<^sub>Ara. \<Gamma>' *  R ra r * \<up> (ra \<in> dom M) * true)"
+    using mod_ex_dist by blast
+  have H: "pHeap (the \<sigma>) (new_addrs h as (the \<sigma>)) (n - t) \<Turnstile> \<Gamma>' * (\<exists>\<^sub>Ara. R ra r * \<up> (ra \<in> dom M)) * true" 
+    apply(rule entailsD[OF _ H']) by auto2
+
+  from ii ie nf have T: "t \<le> n " by auto
+
+  show ?case
+    apply safe
+    subgoal using F by auto
+    subgoal using H by simp  
+    subgoal by fact
+     apply fact apply fact done
+qed
 
 
 
